Changing memAtomic to use nativeFifo, wip

examples/ProcDecSC.v
@@ -32,37 +32,20 @@ Section ProcDecSC.
     "processLd" |-> "execLd";
     "processSt" |-> "execSt"; ||.
 
-  Lemma pdec_pinst_regMap_type:
-    forall ir (Hr: reachable ir (fst (ProcDecInl.pdecInl dec execState execNextPc))),
-      match M.find "Outs"--"elt" ir with
-      | Some s => projT1 s = @NativeKind (listEltT RsToProc type) nil
-      | None => False
-      end.
+  Definition pdec_pinst_regRel (ir sr: RegsT): Prop.
   Proof.
-    abstract (
-        intros; pose proof (procDec_inv_0_ok Hr);
-        unfold procDec_inv_0 in H; dest;
-        rewrite H3; reflexivity).
-  Defined.
-
-  Definition pdec_pinst_regMap (ir: RegsT)
-             (Hr: reachable ir (fst (ProcDecInl.pdecInl dec execState execNextPc))): RegsT.
-  Proof.
-    kgetv "pc"%string pcv ir (Bit addrSize) (M.empty (sigT (fullType type))).
-    kgetv "rf"%string rfv ir (Vector (Data lgDataBytes) rfIdx) (M.empty (sigT (fullType type))).
-
-    pose proof (pdec_pinst_regMap_type Hr) as Hoeltv; clear Hr.
-    destruct (M.find "Outs"--"elt" ir) as [oeltv|]; [|inv Hoeltv].
-    destruct oeltv as [oeltk oeltv].
-    simpl in Hoeltv; subst.
+    kgetv "pc"%string pcv ir (Bit addrSize) False.
+    kgetv "rf"%string rfv ir (Vector (Data lgDataBytes) rfIdx) False.
+    refine (exists oeltv: fullType type (listEltK RsToProc type),
+               M.find "Outs"--"elt" ir = Some (existT _ _ oeltv) /\ _).
 
     pose proof (evalExpr (dec _ rfv pcv)) as inst.
     refine (match oeltv with
-            | nil => M.add "pc"%string (existT _ _ pcv)
-                           (M.add "rf"%string (existT _ _ rfv)
-                                  (M.empty _))
-            | _ => M.add "pc"%string (existT _ _ (evalExpr (execNextPc _ rfv pcv inst)))
-                         (M.add "rf"%string _ (M.empty _))
+            | nil => sr = M.add "pc"%string (existT _ _ pcv)
+                                (M.add "rf"%string (existT _ _ rfv)
+                                       (M.empty _))
+            | _ => sr = M.add "pc"%string (existT _ _ (evalExpr (execNextPc _ rfv pcv inst)))
+                              (M.add "rf"%string _ (M.empty _))
             end).
 
     pose proof (inst ``"opcode") as opc.
@@ -73,41 +56,47 @@ Section ProcDecSC.
                       else rfv a).
     - refine (existT _ _ rfv).
   Defined.
-  Hint Unfold pdec_pinst_regMap: MethDefs. (* for kdecompose_regMap_init *)
-
-  Require Import ProofIrrelevance.
-
-  Ltac pdec_refines_pinst_tac :=
-    kinv_or3;
-    repeat
-      match goal with
-      | [ |- context [pdec_pinst_regMap_type ?Hr] ] =>
-        let Hpf := fresh "Hpf" in
-        assert (Hpf: pdec_pinst_regMap_type Hr = eq_refl) by apply proof_irrelevance;
-        simpl in Hpf; rewrite Hpf
-      end.
+  Hint Unfold pdec_pinst_regRel: MethDefs. (* for kdecompose_regMap_init *)
+  Hint Unfold evalConstT: MethDefs.
   
   Lemma pdec_refines_pinst: pdec <<== pinst.
-  Proof. (* SKIP_PROOF_ON
+  Proof. (* SKIP_PROOF_ON *)
     kinline_left pdeci.
 
-    subst.
-    apply decompositionZeroE with (thetaE:= pdec_pinst_regMap) (ruleMap:= pdec_pinst_ruleMap);
+    apply decompositionZeroR
+    with (thetaR:= pdec_pinst_regRel) (ruleMap:= pdec_pinst_ruleMap);
       intros; subst.
 
     - unfold initRegs, getRegInits; simpl.
       kregmap_red.
       kinv_magic_light_with pdec_refines_pinst_tac.
 
+    - admit.
+      
     - auto.
     - auto.
 
     - pose proof (procDec_inv_0_ok Hreach).
       pose proof (procDec_inv_1_ok Hreach).
+      kinv_add_end.
 
-      admit.
-      kinvert; kinv_magic_with kinv_or3.
-      END_SKIP_PROOF_ON *) admit.
+      kinvert.
+      + kinv_magic_light_with kinv_or3.
+      + kinv_magic_light_with kinv_or3.
+      + kinv_magic_light_with kinv_or3.
+        kinv_finish.
+      + kinv_magic_light_with kinv_or3.
+        kinv_finish.
+      + kinv_magic_light_with kinv_or3.
+        kinv_finish.
+      + kinv_magic_light_with kinv_or3.
+        kinv_finish.
+      + admit.
+      + kinv_magic_light_with kinv_or3.
+        * kinv_finish.
+        * boundedMapTac; kinv_finish.
+        * kinv_finish.
+          (* END_SKIP_PROOF_ON *) admit.
   Qed.
 
 End ProcDecSC.
